Logic/Modal/Standard/Kripke/Completeness.lean
@@ -164,9 +164,8 @@ lemma complete_of_mem_canonicalFrame [Inhabited (Axᴺ)-MCT] {𝔽 : FrameClass.
   . use (CanonicalModel Ax).Valuation;
     exact iff_valid_on_canonicalModel_deducible.not.mpr h;
 
-instance instComplete_of_mem_canonicalFrame [Inhabited (Axᴺ)-MCT] {𝔽 : FrameClass.Dep α} (hFC : ⟨(Axᴺ)-MCT, CanonicalFrame Ax⟩ ∈ 𝔽) : Complete (Axᴺ) 𝔽 := ⟨complete_of_mem_canonicalFrame hFC⟩
+lemma instComplete_of_mem_canonicalFrame [Inhabited (Axᴺ)-MCT] {𝔽 : FrameClass.Dep α} (hFC : ⟨(Axᴺ)-MCT, CanonicalFrame Ax⟩ ∈ 𝔽) : Complete (Axᴺ) 𝔽 := ⟨complete_of_mem_canonicalFrame hFC⟩
 
--- LO.Modal.Standard.Kripke.completeness_of_K.{u_1} {α : Type u_1} [DecidableEq α] : Complete 𝐊 (AllFrameClass.Dep α)
 instance K_complete : Complete 𝐊 AllFrameClass[α] := by
   simpa [←Normal.isK] using instComplete_of_mem_canonicalFrame (Ax := 𝗞) (𝔽 := AllFrameClass[α]) trivial;
 
