Logic/Modal/Standard/PLoN/Completeness.lean
@@ -5,24 +5,23 @@ namespace LO.Modal.Standard
 
 namespace PLoN
 
-variable [DecidableEq α]
+variable {α : Type*} [DecidableEq α]
 
 open Formula
 open Theory
 open MaximalConsistentTheory
 
-abbrev CanonicalFrameN : PLoN.Frame α where
-  World := (𝐍)-MCT
+abbrev CanonicalFrame (Λ : DeductionParameter α) [Inhabited (Λ)-MCT] : PLoN.Frame (Λ)-MCT α where
   Rel :=  λ p Ω₁ Ω₂ => ~(□p) ∈ Ω₁.theory ∧ ~p ∈ Ω₂.theory
 
-abbrev CanonicalModelN : PLoN.Model α where
-  Frame := CanonicalFrameN
+abbrev CanonicalModel (Λ : DeductionParameter α) [Inhabited (Λ)-MCT] : PLoN.Model (Λ)-MCT α where
+  Frame := CanonicalFrame Λ
   Valuation Ω a := (atom a) ∈ Ω.theory
 
-@[reducible]
-instance : Semantics (Formula α) (CanonicalModelN (α := α)).World := Formula.plon_satisfies.instSemantics (CanonicalModelN)
+variable {Λ : DeductionParameter α} [Inhabited (Λ)-MCT] [Λ.HasNec]
+         {p : Formula α}
 
-lemma truthlemma {p : Formula α} : ∀ {Ω : (CanonicalModelN).World}, Ω ⊧ p ↔ (p ∈ Ω.theory) := by
+lemma truthlemma : ∀ {Ω : (CanonicalModel Λ).World}, Ω ⊧ p ↔ (p ∈ Ω.theory) := by
   induction p using Formula.rec' with
   | hbox p ih =>
     intro Ω;
@@ -33,7 +32,7 @@ lemma truthlemma {p : Formula α} : ∀ {Ω : (CanonicalModelN).World}, Ω ⊧ p
       simp [plon_satisfies];
       constructor;
       . assumption;
-      . obtain ⟨Ω', hΩ'⟩ := lindenbaum (𝓓 := 𝐍) (T := {~p}) (not_singleton_consistent Ω.consistent (iff_mem_neg.mpr hC));
+      . obtain ⟨Ω', hΩ'⟩ := lindenbaum (𝓓 := Λ) (T := {~p}) (not_singleton_consistent Ω.consistent (iff_mem_neg.mpr hC));
         use Ω';
         constructor;
         . apply iff_mem_neg.mp;
@@ -47,16 +46,15 @@ lemma truthlemma {p : Formula α} : ∀ {Ω : (CanonicalModelN).World}, Ω ⊧ p
       simp_all only [plon_satisfies.iff_models];
   | _ => simp_all [plon_satisfies];
 
-lemma complete!_on_N {p : Formula α} : ℕ𝔽(𝐍) ⊧ p → 𝐍 ⊢! p:= by
+lemma complete_of_mem_canonicalFrame {𝔽 : FrameClass α} (hFC : ⟨(Λ)-MCT, CanonicalFrame Λ⟩ ∈ 𝔽) : 𝔽 ⊧ p → Λ ⊢! p:= by
   simp [valid_on_PLoNFrameClass, valid_on_PLoNFrame, valid_on_PLoNModel];
-  contrapose;
-  push_neg;
+  contrapose; push_neg;
   intro h;
-  use CanonicalModelN.Frame;
+  use (Λ)-MCT, (CanonicalFrame Λ);
   constructor;
-  . apply Definability.defines' Definability.N |>.mpr; trivial;
-  . use CanonicalModelN.Valuation;
-    obtain ⟨Ω, hΩ⟩ := lindenbaum (𝓓 := 𝐍) (T := {~p}) (by
+  . exact hFC;
+  . use (CanonicalModel Λ).Valuation;
+    obtain ⟨Ω, hΩ⟩ := lindenbaum (𝓓 := Λ) (T := {~p}) (by
       apply unprovable_iff_singleton_neg_Consistent.mp;
       exact h;
     );
@@ -65,7 +63,9 @@ lemma complete!_on_N {p : Formula α} : ℕ𝔽(𝐍) ⊧ p → 𝐍 ⊢! p:= by
     apply iff_mem_neg.mp;
     simp_all;
 
-instance : Complete (𝐍 : DeductionParameter α) ℕ𝔽(𝐍) := ⟨complete!_on_N⟩
+lemma instComplete_of_mem_canonicalFrame {𝔽 : FrameClass α} (hFC : ⟨(Λ)-MCT, CanonicalFrame Λ⟩ ∈ 𝔽) : Complete Λ 𝔽 := ⟨complete_of_mem_canonicalFrame hFC⟩
+
+instance : Complete 𝐍 (AllFrameClass α) := instComplete_of_mem_canonicalFrame trivial
 
 end PLoN
 
