Logic/Modal/Standard/PLoN/Semantics.lean
@@ -6,56 +6,65 @@ namespace LO.Modal.Standard
 
 namespace PLoN
 
-protected structure Frame (α) where
-  World : Type u
-  World_nonempty : Nonempty World := by infer_instance
-  Rel : Formula α → World → World → Prop
+structure Frame (δ α) where
+  [δ_inhabited : Inhabited δ]
+  Rel : Formula α → δ → δ → Prop
 
-instance (F : PLoN.Frame α) : Nonempty F.World := F.World_nonempty
+abbrev Frame.World (_ : PLoN.Frame δ α) := δ
 
-abbrev Frame.Rel' {F : PLoN.Frame α} (p : Formula α) (w w' : F.World) := F.Rel p w w'
+abbrev Frame.default {F : PLoN.Frame δ α} : F.World := F.δ_inhabited.default
+scoped notation "﹫" => Frame.default
+
+
+instance : CoeFun (PLoN.Frame δ α) (λ F => Formula α → F.World → F.World → Prop) := ⟨Frame.Rel⟩
+
+abbrev Frame.Rel' {F : PLoN.Frame δ α} (p : Formula α) (x y : F.World) := F.Rel p x y
 scoped notation:45 x:90 " ≺[" p "] " y:90 => Frame.Rel' p x y
 
-protected structure FiniteFrame (α) extends PLoN.Frame α where
-  World_finite : Finite World := by infer_instance
 
-protected abbrev FrameClass (α) := Set (PLoN.Frame α)
+structure FiniteFrame (δ α) extends Frame δ α where
+  [δ_finite : Finite δ]
 
-protected abbrev FiniteFrameClass (α) := Set (PLoN.FiniteFrame α)
-
-abbrev FrameCondition (α) := PLoN.Frame α → Prop
-
-abbrev FiniteFrameCondition (α) := PLoN.FiniteFrame α → Prop
+instance : Coe (FiniteFrame δ α) (Frame δ α) := ⟨λ F ↦ F.toFrame⟩
 
 
-abbrev Valuation (W : Type u) (α : Type u) := W → α → Prop
+abbrev TerminalFrame (α) : FiniteFrame (Fin 1) α where
+  Rel := λ _ _ _ => True
 
-protected structure Model (α) where
-  Frame : PLoN.Frame α
-  Valuation : Valuation Frame.World α
 
-abbrev Model.World (M : PLoN.Model α) := M.Frame.World
-instance : CoeSort (PLoN.Model α) (Type _) where coe := Model.World
+abbrev FrameClass (α : Type*) := Set ((δ : Type*) × PLoN.Frame δ α)
+
+
+abbrev Valuation (F : PLoN.Frame δ α) (α : Type*) := F.World → α → Prop
+
+structure Model (δ α) where
+  Frame : PLoN.Frame δ α
+  Valuation : PLoN.Valuation Frame α
+
+abbrev Model.World (M : PLoN.Model δ α) := M.Frame.World
+instance : CoeSort (PLoN.Model δ α) (Type _) := ⟨Model.World⟩
 
 end PLoN
 
+variable {δ α : Type*}
+
 open Standard.PLoN
 
-def Formula.plon_satisfies (M : PLoN.Model α) (w : M.World) : Formula α → Prop
+def Formula.plon_satisfies (M : PLoN.Model δ α) (w : M.World) : Formula α → Prop
   | atom a  => M.Valuation w a
   | verum   => True
   | falsum  => False
   | and p q => (p.plon_satisfies M w) ∧ (q.plon_satisfies M w)
   | or p q  => (p.plon_satisfies M w) ∨ (q.plon_satisfies M w)
   | imp p q => (p.plon_satisfies M w) → (q.plon_satisfies M w)
-  | box p   => ∀ w', w ≺[p] w' → (p.plon_satisfies M w')
+  | box p   => ∀ {w'}, w ≺[p] w' → (p.plon_satisfies M w')
 
 
 namespace Formula.plon_satisfies
 
-protected instance instSemantics (M : PLoN.Model α) : Semantics (Formula α) (M.World) := ⟨fun w ↦ Formula.plon_satisfies M w⟩
+protected instance semantics (M : PLoN.Model δ α) : Semantics (Formula α) (M.World) := ⟨fun w ↦ Formula.plon_satisfies M w⟩
 
-variable {M : PLoN.Model α} {w : M.World} {p q : Formula α}
+variable {M : PLoN.Model δ α} {w : M.World} {p q : Formula α}
 
 @[simp] protected lemma iff_models : w ⊧ p ↔ p.plon_satisfies M w := by rfl
 
@@ -70,90 +79,105 @@ instance : Semantics.Tarski M.World where
 end Formula.plon_satisfies
 
 
-def Formula.valid_on_PLoNModel (M : PLoN.Model α) (p : Formula α) : Prop := ∀ w : M.World, w ⊧ p
+def Formula.valid_on_PLoNModel (M : PLoN.Model δ α) (p : Formula α) : Prop := ∀ w : M.World, w ⊧ p
 
 namespace Formula.valid_on_PLoNModel
 
-instance : Semantics (Formula α) (PLoN.Model α) := ⟨fun M ↦ Formula.valid_on_PLoNModel M⟩
+instance : Semantics (Formula α) (PLoN.Model δ α) := ⟨fun M ↦ Formula.valid_on_PLoNModel M⟩
 
 @[simp]
-protected lemma Formula.valid_on_PLoNModel.iff_models {M : PLoN.Model α} {p : Formula α}
+protected lemma iff_models {M : PLoN.Model δ α} {p : Formula α}
 : M ⊧ p ↔ Formula.valid_on_PLoNModel M p := by rfl
 
-instance : Semantics.Bot (PLoN.Model α) where
-  realize_bot _ := by simp [Formula.valid_on_PLoNModel];
+instance : Semantics.Bot (PLoN.Model δ α) where
+  realize_bot _ := by
+    simp [Formula.valid_on_PLoNModel];
+    use ﹫;
 
 end Formula.valid_on_PLoNModel
 
 
-def Formula.valid_on_PLoNFrame (F : PLoN.Frame α) (p : Formula α) := ∀ V, (Model.mk F V) ⊧ p
+def Formula.valid_on_PLoNFrame (F : PLoN.Frame δ α) (p : Formula α) := ∀ V, (Model.mk F V) ⊧ p
 
 namespace Formula.valid_on_PLoNFrame
 
-instance : Semantics (Formula α) (PLoN.Frame α) := ⟨fun F ↦ Formula.valid_on_PLoNFrame F⟩
+instance : Semantics (Formula α) (PLoN.Frame δ α) := ⟨fun F ↦ Formula.valid_on_PLoNFrame F⟩
 
 @[simp]
-protected lemma Formula.valid_on_PLoNFrame.iff_models {F : PLoN.Frame α} {p : Formula α}
+protected lemma iff_models {F : PLoN.Frame δ α} {p : Formula α}
 : F ⊧ p ↔ Formula.valid_on_PLoNFrame F p := by rfl
 
-instance : Semantics.Bot (PLoN.Frame α) where
+variable {F : Frame δ α}
+
+instance : Semantics.Bot (PLoN.Frame δ α) where
   realize_bot _ := by simp [Formula.valid_on_PLoNFrame];
+
+protected lemma nec (h : F ⊧ p) : F ⊧ □p := by
+  intro V x y _;
+  exact h V y;
+
+protected lemma mdp (hpq : F ⊧ p ⟶ q) (hp : F ⊧ p) : F ⊧ q := by
+  intro V x;
+  exact (hpq V x) (hp V x);
 
 end Formula.valid_on_PLoNFrame
 
 
-def Formula.valid_on_PLoNFrameClass (𝔽 : PLoN.FrameClass α) (p : Formula α) := ∀ (F : PLoN.Frame α), F ∈ 𝔽 → F ⊧ p
+def Formula.valid_on_PLoNFrameClass (𝔽 : PLoN.FrameClass α) (p : Formula α) := ∀ {δ F}, ⟨δ, F⟩ ∈ 𝔽 → F ⊧ p
 
 namespace Formula.valid_on_PLoNFrameClass
 
 instance : Semantics (Formula α) (PLoN.FrameClass α) := ⟨fun 𝔽 ↦ Formula.valid_on_PLoNFrameClass 𝔽⟩
 
+variable {𝔽 : FrameClass α}
+
 @[simp]
-protected lemma Formula.valid_on_PLoNFrameClass.iff_models {𝔽 : PLoN.FrameClass α} {p : Formula α}
-: 𝔽 ⊧ p ↔ Formula.valid_on_PLoNFrameClass 𝔽 p := by rfl
+protected lemma iff_models {𝔽 : PLoN.FrameClass α} {p : Formula α} : 𝔽 ⊧ p ↔ Formula.valid_on_PLoNFrameClass 𝔽 p := by rfl
+
+protected lemma nec (h : 𝔽 ⊧ p) : 𝔽 ⊧ □p := by
+  intro _ _ hF;
+  apply valid_on_PLoNFrame.nec;
+  exact h hF;
+
+protected lemma mdp (hpq : 𝔽 ⊧ p ⟶ q) (hp : 𝔽 ⊧ p) : 𝔽 ⊧ q := by
+  intro _ _ hF;
+  exact valid_on_PLoNFrame.mdp (hpq hF) (hp hF)
 
 end Formula.valid_on_PLoNFrameClass
 
 
+def DeductionParameter.DefinesPLoNFrameClass (𝓓 : DeductionParameter α) (𝔽 : PLoN.FrameClass α) := ∀ {δ}, ∀ {F : Frame δ α}, F ⊧* 𝓓.theory ↔ ⟨δ, F⟩ ∈ 𝔽
+
 namespace PLoN
 
-notation "Th(" 𝓓 ")" => System.theory 𝓓
 
-def DeductionParamterFrameClass (𝓓 : DeductionParameter α) : PLoN.FrameClass α := { F : PLoN.Frame α | F ⊧* Th(𝓓) }
-notation "ℕ𝔽(" 𝓓 ")" => PLoN.DeductionParamterFrameClass 𝓓
+abbrev AllFrameClass (α) : FrameClass α := Set.univ
 
-
-class Definability (𝓓 : DeductionParameter α) (P : FrameCondition α) where
-  defines : ∀ {F}, F ⊧* Th(𝓓) ↔ P F
-
-lemma Definability.defines' (definability : Definability 𝓓 P) : ∀ {F}, F ∈ ℕ𝔽(𝓓) ↔ P F := definability.defines
+lemma AllFrameClass.nonempty : (AllFrameClass.{_, 0} α).Nonempty := by
+  use ⟨Fin 1, TerminalFrame α⟩
+  trivial;
 
 open Formula
 
-instance Definability.N : Definability (α := α) 𝐍 (λ _ => True) where
-  defines := by
-    simp [System.theory, valid_on_PLoNFrame, valid_on_PLoNModel];
-    intro F p hp;
-    induction hp using Deduction.inducition_with_necOnly! with
-    | hMaxm h => simp at h;
-    | hMdp ihpq ihp =>
-      intro V w;
-      exact (ihpq V w) (ihp V w)
-    | hNec ihp =>
-      intro V w w' _;
-      exact ihp V w';
-    | hDisj₃ =>
-      simp_all only [plon_satisfies];
-      intros; rename_i hpr hqr hpq;
-      cases hpq with
-      | inl hp => exact hpr hp;
-      | inr hq => exact hqr hq;
-    | _ => simp_all [plon_satisfies];
-
-lemma FrameClassNonempty.N : Set.Nonempty (ℕ𝔽(𝐍) : PLoN.FrameClass α) := by
-  existsi {World := PUnit, Rel := λ _ _ _ => True};
-  apply Definability.defines' Definability.N |>.mpr;
-  trivial;
+lemma N_defines : 𝐍.DefinesPLoNFrameClass (AllFrameClass α) := by
+  intro δ F;
+  simp [DeductionParameter.theory, System.theory, valid_on_PLoNFrame, valid_on_PLoNModel];
+  intro p hp;
+  induction hp using Deduction.inducition_with_necOnly! with
+  | hMaxm h => simp at h;
+  | hMdp ihpq ihp =>
+    intro V w;
+    exact (ihpq V w) (ihp V w)
+  | hNec ihp =>
+    intro V w w' _;
+    exact ihp V w';
+  | hDisj₃ =>
+    simp_all only [plon_satisfies];
+    intros; rename_i hpr hqr hpq;
+    cases hpq with
+    | inl hp => exact hpr hp;
+    | inr hq => exact hqr hq;
+  | _ => simp_all [plon_satisfies];
 
 end PLoN
 
